CBPV/Normalization.lean
@@ -39,8 +39,8 @@ theorem SN_soundness :
   case snecom.app snem _ snm snv => exact .app (.ne snem) snm snv
   case snecom.letin snem _ snm snn => exact .letin (.ne snem) snm snn
   case snecom.case snv _ _ snm snn => exact .case snv snm snn
-  case snecom.prjl snem snm => exact .prjl (.ne snem) snm
-  case snecom.prjr snem snm => exact .prjr (.ne snem) snm
+  case snecom.fst snem snm => exact .fst (.ne snem) snm
+  case snecom.snd snem snm => exact .snd (.ne snem) snm
   case snval.var => constructor; intro _ r; cases r
   case snval.unit => constructor; intro _ r; cases r
   case snval.inl ih => exact .inl ih
@@ -51,17 +51,7 @@ theorem SN_soundness :
   case sncom.prod ihm ihn => exact .prod ihm ihn
   case sncom.ne => assumption
   case sncom.red r ih => exact r.closure ih
-  case srcom.thunk => constructor
-  case srcom.lam => constructor; assumption
-  case srcom.ret => constructor; assumption
-  case srcom.inl => constructor <;> assumption
-  case srcom.inr => constructor <;> assumption
-  case srcom.app => constructor <;> assumption
-  case srcom.letin => constructor <;> assumption
-  case srcom.prodl => constructor <;> assumption
-  case srcom.prodr => constructor <;> assumption
-  case srcom.prjl => constructor <;> assumption
-  case srcom.prjr => constructor <;> assumption
+  all_goals constructor <;> assumption
 
 /-*------------------------------------------
   Well typed terms are strongly normalizing
